chore: normal form cleanup

tests/playground/bool_exhaust_test.lean
@@ -1,439 +1,10 @@
-import Lean.Elab.Command
-import Lean.Elab.Tactic.ElabTerm
-import Lean.Elab.Tactic.Meta
-import Lean.Meta.CheckTactic
-import Lean.Parser.Term
+import Lean.Util.TestNormalForms
 
-open Lean Lean.Meta Lean.Elab Lean.Elab.Term Lean.Elab.Command
-open Lean.Meta.CheckTactic
-
-
--- | A `Op` is a first order operation for generating values with a given type.
-structure Op (tp : Type) (val : Type) where
-  args : Array tp
-  result : tp
-  apply : Array val → val
- deriving Inhabited
-
-def mkOp (args : List tp) (result : tp) (apply : Array val → val) : Op tp val :=
-  { apply := apply, args := args.toArray, result }
-
-def Op.map (op : Op x val) (f : x → y) : Op y val :=
-  { apply := op.apply, args := op.args.map f, result := f op.result }
-
-class HasType (val : Type) (type : outParam Type) where
-  typeOf : val → type
-
-class Value (val : Type) where
-  render : val → TermElabM Term
-
-/--
-Contextual information needed to generate terms.
--/
-structure GenCtx (val : Type) where
-  -- Maps type indices to operator for corresponding type.
-  -- Types use type indices.
-  ops : Array (Array (Op Nat val))
-  /- Operators to use for patterns at top of terms -/
-  topOps : Array (Op Nat val)
-  /-- Maximum term size -/
-  maxTermSize : Nat
-  /-- Maximum depth of terms -/
-  maxDepth : Nat
-  /-- Maximum number of variables -/
-  maxVarCount : Nat
-  /- Local context variables defined in -/
-  lctx : LocalContext
-  /- Local instances for variables -/
-  linst : LocalInstances
-  /-- Maps type indices to variables for that type. -/
-  vars : Array (Array val)
-
-namespace GenCtx
-
-/-- `var ctx tp idx` returns a term denoting `i`th variable with type `tp`. -/
-def var (ctx : GenCtx val) (tp : Nat) (idx : Nat) : Option val :=
-  if g : tp < ctx.vars.size then
-    let a := ctx.vars[tp]'g
-    if h : idx < a.size then
-      some (a[idx]'h)
-    else
-      none
-  else
-    none
-
-end GenCtx
-
-/-- An operator together with a set of terms to apply to it. -/
-structure PartialApp (term : Type) where
-  /-- Operator to generate -/
-  op : Op Nat term
-  /-- Terms constructed so far -/
-  terms : Array term
-
-namespace PartialApp
-
-def fromOp (op : Op Nat term) : PartialApp term :=
-  { op, terms := .mkEmpty op.args.size }
-
-end PartialApp
-
-/--
-A partial term contains the initial part of a term as constructed from a
-left-to-right preorder traversal.
-
-It stores additional information needed to ensure the ultimate term satisfies
-the generation constraints on term size and number of variables.
-
-The operations for constructing this ensures the term is well-formed
-with respect to the signature and is not a complete term.
--/
-structure PartialTerm (term : Type) where
-  /-- Stack of partially built term (must be non-empty) -/
-  termStack : Array (PartialApp term)
-  /-- Maximum number of additional operations that may be added. -/
-  remTermSize : Nat
-  /-- Variables used with type index. -/
-  usedVars : Array Nat
-  deriving Inhabited
-
-namespace PartialTerm
-
-/--
-Create an initial partial term from an operator.
-
-If the operator is a constant, then this just returns a complete terms.
--/
-def init (maxTermSize : Nat) (maxDepth : Nat) (op : Op Nat term) : term ⊕ PartialTerm term :=
-  if op.args.isEmpty then
-    .inl (op.apply #[])
-  else
-    .inr {
-      termStack := #[PartialApp.fromOp op],
-      remTermSize := maxTermSize - (1 + op.args.size),
-      usedVars := #[]
-    }
-
-partial def push (p : PartialTerm term) (t : term) : term ⊕ PartialTerm term :=
-  match p.termStack.back? with
-  | none => .inl t
-  | some { op, terms } =>
-    let p := { p with termStack := p.termStack.pop }
-    let terms := terms.push t
-    if terms.size = op.args.size then
-      let v := op.apply terms
-      push p v
-    else
-      .inr { p with termStack := p.termStack.push { op, terms } }
-
-/-- Push an operator to the stack -/
-def pushOp (p : PartialTerm term) (op : Op Nat term) : PartialTerm term :=
-  { termStack   := p.termStack.push (.fromOp op)
-    remTermSize := p.remTermSize - op.args.size,
-    usedVars := p.usedVars
-  }
-
-end PartialTerm
-
-/--
-Term generator
--/
-structure Gen (term : Type) where
-  sofar : Array term := #[]
-  pending : Array (PartialTerm term) := #[]
-  deriving Inhabited
-
-namespace Gen
-
-/-- Return true if generator will return no more terms. -/
-def isEmpty (s: Gen term) : Bool := s.sofar.isEmpty && s.pending.isEmpty
-
-def pop (s : Gen term) : Option (Nat × PartialTerm term × Gen term) :=
-  if s.pending.isEmpty then
-    .none
-  else
-    let { sofar, pending } := s
-    let next := pending.back
-    let pending := pending.pop
-    match next.termStack.back? with
-    | none =>
-      panic! "Term stack empty"
-    | some app =>
-      let tp := app.op.args[app.terms.size]!
-      some (tp, next, { sofar, pending })
-
-/- `push s next v` adds the result of `next.push v` to the state. -/
-def push (s : Gen term) (next : PartialTerm term) (v : term) : Gen term :=
-  let { sofar, pending } := s
-  match next.push v with
-  | .inl v => { sofar := sofar.push v, pending }
-  | .inr next => { sofar, pending := pending.push next }
-
-def pushOp (s : Gen term) (ctx : GenCtx term) (next : PartialTerm term) (op : Op Nat term) :=
-  if op.args.isEmpty then
-    s.push next (op.apply #[])
-  else if op.args.size ≤ next.remTermSize ∧ next.termStack.size + 1 < ctx.maxDepth then
-    { s with pending := s.pending.push (next.pushOp op) }
-  else
-    s
-
-def add (s : Gen term) (val : term ⊕ PartialTerm term) : Gen term :=
-  let { sofar, pending } := s
-  match val with
-  | .inl v => { sofar := sofar.push v, pending }
-  | .inr p => { sofar, pending := pending.push p }
-
-/-- Create state that will explore all terms in context -/
-def addOpInstances (s : Gen term) (ctx : GenCtx term) (op : Op Nat term) : Gen term :=
-  s.add (PartialTerm.init ctx.maxTermSize ctx.maxDepth op)
-
-/-- Create state that will explore all terms in context -/
-def init (ctx : GenCtx term) : Gen term :=
-  ctx.topOps.foldl (init := {}) (·.addOpInstances ctx ·)
-
-end Gen
-
-/--
-Generate terms until we reach the limit.
--/
-partial
-def generateTerms
-    (ctx : GenCtx term)
-    (s : Gen term)
-    (limit : Nat := 0) :
-    Array term × Gen term :=
-  if limit > 0 ∧ s.sofar.size ≥ limit then
-    (s.sofar, { s with sofar := #[] })
-  else
-    match s.pop with
-    | none => (s.sofar, { s with sofar := #[] })
-    | some (tp, next, s) =>
-      let addVar (next : PartialTerm term) (i : Nat) (s : Gen term) : Gen term :=
-            if next.usedVars[i]! = tp then
-              match ctx.var tp i with
-              | some v => s.push next v
-              | none => s
-            else
-              s
-      let s := next.usedVars.size.fold (init := s) (addVar next)
-      let s :=
-        let var := next.usedVars.size
-        if var < ctx.maxVarCount then
-          let next := { next with usedVars := next.usedVars.push tp }
-          addVar next var s
-        else
-          s
-      generateTerms ctx (ctx.ops[tp]!.foldl (init := s) (·.pushOp ctx next ·))
+open Lean
+open Lean.Elab.Command (CommandElab)
+open Lean.Test.NormalForms
 
 /-
-`addScopeVariables` extends the local context and instances with a copy of the
-variables in the scope (which must be non-empty).
--/
-def addScopeVariables (lctx : LocalContext) (linst : LocalInstances) (scope : Scope) (idx : Nat) :
-    CoreM (LocalContext × LocalInstances × Ident) := do
-  let act := Term.elabBindersEx scope.varDecls fun vars => do pure (vars, ← (read : MetaM Meta.Context))
-  let mctx := { lctx := lctx, localInstances := linst }
-  let (((vars, mctx), _tstate), _mstate) ← act |>.run |>.run mctx
-  if vars.isEmpty then
-    throwError "No variables declared"
-  let fv := vars[0]!.snd |>.fvarId!
-  let rec drop (nm : Name) :=
-        match nm with
-        | .str .anonymous s => pure (.str .anonymous s!"{s}{idx}")
-        | .str nm _ => drop nm
-        | .num nm _ => drop nm
-        | .anonymous => throwError "Anonymous variable declared."
-  let nm ← drop (mctx.lctx.get! fv |>.userName)
-  let lctx := mctx.lctx.setUserName fv nm
-  pure (lctx, mctx.localInstances, mkIdent nm)
-
-def addVariables (cmdCtx : Command.Context) (cmdState : Command.State) (lctx : LocalContext) (linst : LocalInstances) (n : Nat) (cmd : Command) :
-    CoreM (LocalContext × LocalInstances × Array Ident) := do
-  let (_, s) ←  elabCommand cmd.raw |>.run cmdCtx |>.run cmdState
-  let scope := s.scopes.head!
-  Nat.foldM (n := n) (init := (lctx, linst, .mkEmpty n)) fun i (lctx, linst, a) => do
-    let (lctx, linst, ident) ← addScopeVariables lctx linst scope i
-    pure (lctx, linst, a.push ident)
-
-structure VarDecl (tp : Type) where
-  idx : Nat
-  ident : TSyntax `ident
-  type : tp
-  deriving Inhabited, Repr
-
-instance : BEq (VarDecl tp) where
-  beq x y := x.idx == y.idx
-
-instance : Hashable (VarDecl tp) where
-  hash v := hash v.idx
-
-structure GenStats where
-  maxTermSize : Nat := 9
-  maxDepth : Nat := 3
-  maxVarCount : Nat := 3
-
-def mkCtx [BEq tp] [Hashable tp]
-    (types : Array tp)
-    (ops : List (Op tp val))
-    (varGen : List (tp × CoreM Command))
-    (mkVar : VarDecl tp → val)
-    (stats : GenStats)
-    (topOps : List (Op tp val) := ops) : CommandElabM (GenCtx val) := do
-  let typeMap : HashMap tp Nat := Nat.fold (n := types.size) (init := {}) fun i s =>
-        if p : i < types.size then
-          s.insert types[i] i
-        else
-          s
-  let typeFn (t : tp) := typeMap.findD t 0
-  let addOp (a : Array (Array (Op Nat val))) (op : Op tp val) :=
-        let op := op.map typeFn
-        a.modify op.result (·.push op)
-  let init := Array.ofFn (n := types.size) (fun _ => #[])
-  let ops := ops.foldl (init := init) addOp
-  let ops := ops.map (·.reverse)
-  let topOps := topOps.toArray.map (·.map typeFn)
-  let (lctx, linst, vars) ← liftCoreM do
-    let coreCtx ← read
-    let coreState ← get
-    let fileName := coreCtx.fileName
-    let fileMap  := coreCtx.fileMap
-    let env := coreState.env
-    let maxRecDepth := coreCtx.maxRecDepth
-    let cmdCtx : Command.Context := { fileName, fileMap, tacticCache? := none }
-    let cmdState : Command.State := { env, maxRecDepth }
-    let addVars (p : LocalContext × LocalInstances × Array (Array val))
-                (q : tp × CoreM Command) :
-                CoreM (LocalContext × LocalInstances × _) := do
-          let (lctx, linst, a) := p
-          let (type, gen) := q
-          let cmd ← gen
-          let (lctx, linst, vars) ← addVariables cmdCtx cmdState lctx linst stats.maxVarCount cmd
-          let vars := Array.ofFn (n := vars.size) fun j => mkVar { idx := j.val, ident := vars[j], type }
-          let type := typeFn type
-          pure (lctx, linst, a.modify type (fun _ => vars))
-    let vars := Array.ofFn (n := types.size) fun _ => #[]
-    varGen.foldlM (init := ({}, {}, vars)) addVars
-  let maxTermSize : Nat := stats.maxTermSize
-  let maxDepth : Nat := stats.maxDepth
-  let maxVarCount : Nat := stats.maxVarCount
-  pure { ops, topOps, maxTermSize, maxDepth, maxVarCount, lctx, linst, vars }
-
-def runTests [BEq tp] [HasType val tp] [Value val] (stx : Syntax) (simp : val → val)(tac : Syntax.Tactic) (terms : Array val)
-      : TermElabM Unit := do
-  for tm in terms do
-    if ← IO.checkCanceled then
-      -- should never be visible to users!
-      throw <| Exception.error .missing "Testing interrupted"
-    let res := simp tm
-    let t ← Value.render tm
-    if HasType.typeOf tm != HasType.typeOf res then
-      throwErrorAt stx m!"simp spec for {t} did not preserve type."
-    withoutModifyingEnv $ do
-      let exp ← Value.render res
-      let u ← Lean.Elab.Term.elabTerm t none
-      let type ← inferType u
-      let checkGoalType ← mkCheckGoalType u type
-      let expTerm ← Lean.Elab.Term.elabTerm exp (some type)
-      let mvar ← mkFreshExprMVar (.some checkGoalType)
-      let (goals, _) ← Lean.Elab.runTactic mvar.mvarId! tac.raw
-      match goals with
-      | [next] => do
-        let (val, _, _) ← matchCheckGoalType stx (←next.getType)
-        if !(← Meta.withReducible <| isDefEq val expTerm) then
-          logErrorAt stx
-            m!"{indentExpr u} reduces to{indentExpr val}\nbut is expected to reduce to {indentExpr expTerm}"
-      | [] =>
-        logErrorAt stx
-          m!"{tac} closed goal, but is expected to reduce to {indentExpr expTerm}."
-      | _ => do
-        logErrorAt stx
-          m!"{tac} produced multiple goals, but is expected to reduce to {indentExpr expTerm}."
-
-private def mkCoreContext (ctx : Command.Context) (options : Options) (maxRecDepth : Nat) (initHeartbeats : Nat) : Core.Context :=
-  { fileName       := ctx.fileName
-    fileMap        := ctx.fileMap
-    options,
-    currRecDepth   := ctx.currRecDepth
-    maxRecDepth,
-    ref            := ctx.ref
-    initHeartbeats,
-    currMacroScope := ctx.currMacroScope }
-
-/-- Runs term elaborator in base context. -/
-def runTermElabM (cctx : Core.Context) (cstate : Core.State) (mctx : Meta.Context) (act : TermElabM Unit)
-    : BaseIO (Except Exception MessageLog) := do
-  let r ← act.run |>.run mctx |>.run cctx cstate |>.toBaseIO
-  match r with
-  | .error e =>
-    pure (.error e)
-  | .ok ((((), _termS), _metaS), coreS) =>
-    pure (.ok coreS.messages)
-
-partial
-def runGen [BEq tp] [Hashable tp] [HasType term tp] [Value term]
-
-      (stx : Syntax) (simp : term → term)
-      (varGen : List (tp × CoreM Command))
-      (mkVar : VarDecl tp → term)
-      (stats : GenStats)
-      (types : Array tp)
-      (ops : List (Op tp term))
-      (tac : Syntax.Tactic)
-      (topOps : List (Op tp term) := ops)
-      (concurrent : Bool := true) : CommandElabM Unit := do
-
-  let ctx ← mkCtx (types := types) (ops := ops) (topOps := topOps) (varGen := varGen) (mkVar := mkVar) (stats := stats)
-
-  let lctx := ctx.lctx
-  let linst := ctx.linst
-
-  let cmdCtx : Command.Context ← read
-  let s ← get
-  let ngen := s.ngen
-  let env := s.env
-  let maxRecDepth := s.maxRecDepth
-  let heartbeats ← IO.getNumHeartbeats
-  let options ← getOptions
-  let cctx := mkCoreContext cmdCtx options maxRecDepth heartbeats
-  let cstate : Core.State := { env := env, ngen := ngen, infoState.enabled := false }
-  let mctx : Meta.Context := { lctx := lctx, localInstances := linst }
-  let gen := Gen.init ctx
-  if concurrent then
-    let limit := 400
-    let rec loop (gen : Gen term) (tasks : Array (Task (Except Exception MessageLog))) := do
-      if gen.isEmpty then
-        return tasks
-      else
-        IO.println s!"Writing task"
-        let (terms, gen) := generateTerms ctx gen (limit := limit)
-        let t ← runTests stx simp tac terms |> runTermElabM cctx cstate mctx |>.asTask
-        loop gen (tasks.push t)
-    let tasks ←
-      profileitM Exception "simptest.launch" ({} : Options) (decl := .anonymous) do
-        loop gen #[]
-
-    profileitM Exception "simptest.execute" {} do
-      for i in [0:tasks.size] do
-        if ← IO.checkCanceled then
-          break
-        let act := tasks[i]!
-        match act.get with
-        | .error e =>
-          -- Cancel all tasks after this one
-          (tasks |>.toSubarray (start := i+1) |>.forM IO.cancel : BaseIO Unit)
-          throw e
-        | .ok m =>
-          modify fun s => { s with messages := s.messages ++ m }
-  else
-    let r ← runTermElabM cctx cstate mctx <|
-      let (terms, _) := generateTerms ctx gen
-      runTests stx simp tac terms
-    match r with
-    | .error e => throw e
-    | .ok m => modify fun s => { s with messages := s.messages ++ m }
-
-/-
-
 This file runs many tests on simp and other operations on Boolean/Prop
 values.
 
@@ -596,7 +167,6 @@ def map (f : BoolVal -> BoolVal) (v : BoolVal) : BoolVal :=
   | .ne x y op => .ne (f x) (f y) op
   | .ite c x y op => .ite (f c) (f x) (f y) op
 
-
 def trueProp  : BoolVal := .trueVal .prop
 def falseProp : BoolVal := .falseVal .prop
 def trueBool  : BoolVal := .trueVal .bool
@@ -639,7 +209,6 @@ def coerceType (v : BoolVal) (type : BoolType) : BoolVal :=
   | .bool, .prop => eq_true v
   | _, _ => v
 
-
 /--
 Returns true if we should consider `x` a complement of `y`.
 
@@ -654,7 +223,6 @@ def isComplement (x y : BoolVal) : Bool :=
   | eq_true x, eq_false y => x == y
   | eq_false x, eq_true y => x == y
   | _, _ => false
-
 
 def resolveEq (thunks : List (term → term → Option term)) (x y : term) : Option term :=
   match thunks with
@@ -679,6 +247,14 @@ def isOrComplement (x y : BoolVal) (tp : BoolType) : Bool :=
   | eq_false x, eq_true y, _ => x == y
   | _, _, _ => false
 
+namespace BoolVal
+
+open BoolType
+
+variable (tp : BoolType)
+
+end BoolVal
+
 partial def simp (v : BoolVal) : BoolVal :=
   let v := map simp v
   match v with
@@ -687,8 +263,6 @@ partial def simp (v : BoolVal) : BoolVal :=
       match p with
       | .trueVal  _ => .trueVal  .bool
       | .falseVal _ => .falseVal .bool
-      | .var _ => v
-      | .boolToProp _ => panic! "Expected boolToProp to simplify away"
       | .not x _   => simp <| ~(.decide x)
       | .and x y _ => simp <| (.decide x) &&& (.decide y)
       | .or x y _  => simp <| (.decide x) ||| (.decide y)
@@ -708,6 +282,8 @@ partial def simp (v : BoolVal) : BoolVal :=
         match op with
         | .iteProp => simp <| .ite c (.decide t) (.decide f) .iteBool
         | _ => v
+      | .var _ => v
+      | .boolToProp _ => panic! "Expected boolToProp to simplify away"
       | .decide _ | .eq _ _ _ =>
         panic! s!"Unexpected prop {repr p} when bool expected."
   | .not t _ =>
@@ -780,7 +356,6 @@ partial def simp (v : BoolVal) : BoolVal :=
     | .falseVal _, _ => .trueVal .prop
     | _, .trueVal _ => y
     | _, .falseVal _ => simp <| .not x .prop
-    | .and a b _, y => simp <| .implies a (.implies b y)
     | x, y => Id.run <| do
       if x == y then
         return (.trueVal .prop)
@@ -798,7 +373,8 @@ partial def simp (v : BoolVal) : BoolVal :=
       if let .not yn _ := y then
         if x == yn then
           return y
-
+      if let .and a b _ := x then
+        return simp <| .implies a <| .implies b y
       return v
   | .eq (.trueVal _) y op =>
     match y with
@@ -1035,11 +611,10 @@ set_option profiler false
 
 end BoolVal
 
-instance : HasType BoolVal BoolType where
-  typeOf val := val.typeOf
-
-instance : Value BoolVal where
-  render val := val.render
+def vars : List (BoolType × CoreM Command) := [
+    (.bool, `(variable (b : Bool))),
+    (.prop, `(variable (p : Prop) [Decidable p]))
+  ]
 
 section
 open BoolVal BoolType
@@ -1047,29 +622,27 @@ open BoolVal BoolType
 def trueOp  (tp : BoolType) := mkOp [] tp fun _ => trueVal  tp
 def falseOp (tp : BoolType) := mkOp [] tp fun _ => falseVal tp
 def boolToPropOp := mkOp [.bool] prop fun a => boolToProp (a[0]!)
-def propToBoolOp := mkOp [prop] bool fun a => BoolVal.decide (a[0]!)
-
+def propToBoolOp := mkOp [prop] .bool fun a => BoolVal.decide (a[0]!)
 def notOp (tp : BoolType) := mkOp [tp] tp fun a => not (a[0]!) tp
 def andOp (tp : BoolType) := mkOp [tp, tp] tp fun a => and (a[0]!) (a[1]!) tp
 def orOp  (tp : BoolType) := mkOp [tp, tp] tp fun a => or  (a[0]!) (a[1]!) tp
 def impliesOp := mkOp [.prop, .prop] prop fun a => implies  (a[0]!) (a[1]!)
-def eqOp  (op : EqOp)  :=
-  mkOp [op.argType, op.argType] op.resultType fun a => eq (a[0]!) (a[1]!) op
-def neOp  (op : NeOp)  :=
-  mkOp [op.argType, op.argType] op.resultType fun a => ne (a[0]!) (a[1]!) op
+def eqOp (op : EqOp) := mkOp [op.argType, op.argType] op.resultType fun a => eq (a[0]!) (a[1]!) op
+def neOp (op : NeOp) := mkOp [op.argType, op.argType] op.resultType fun a => ne (a[0]!) (a[1]!) op
 def iteOp (op : IteOp) :=
   let rtp := op.resultType
   mkOp [op.condType, rtp, rtp] rtp fun a => ite (a[0]!) (a[1]!) (a[2]!) op
 
 end
 
-def mkBoolDecl : CoreM Command := `(variable (b : Bool))
-def mkDecidablePropDecl : CoreM Command := `(variable (p : Prop) [Decidable p])
+instance : GenTerm BoolVal BoolType where
+  mkVar := BoolVal.var
+  render := BoolVal.render
 
 syntax:lead (name := boolTestElab) "#boolTest" : command
 
 @[command_elab boolTestElab]
-def elabGenTest : CommandElab := fun stx => do
+def elabBoolTest : CommandElab := fun _stx => do
   let baseOps := [
       trueOp  .bool,  trueOp .prop,
       falseOp .bool, falseOp .prop,
@@ -1086,15 +659,13 @@ def elabGenTest : CommandElab := fun stx => do
     --iteOp .diteProp,  iteOp .diteBool,
     iteOp .condBool
   ]
-  let types := #[.prop, .bool]
+  let types := [.prop, .bool]
   let ops := baseOps ++ eqOps ++ neOps ++ iteOps
-  let varGen : List (BoolType × CoreM Command) := [
-      (.bool, mkBoolDecl),
-      (.prop, mkDecidablePropDecl)
-  ]
   let stats : GenStats := { maxTermSize := 7, maxDepth := 3, maxVarCount := 2 }
-  let tac : Syntax.Tactic ← `(tactic|try simp)
-  runGen stx BoolVal.simp varGen BoolVal.var stats types ops (topOps := ops) tac
+  testNormalForms types ops vars BoolVal.simp stats
 
 set_option maxHeartbeats 10000000
+--set_option profiler true
+--set_option profiler.threshold 1
+set_option trace.Test.normalforms true
 #boolTest
