src/Lean/Util.lean
@@ -25,6 +25,7 @@ import Lean.Util.ReplaceLevel
 import Lean.Util.FoldConsts
 import Lean.Util.SCC
 import Lean.Util.TestExtern
+import Lean.Util.TestNormalForms
 import Lean.Util.OccursCheck
 import Lean.Util.HasConstCache
 import Lean.Util.FileSetupInfo
