src/Lean/Util/TestNormalForms.lean
@@ -1,0 +1,493 @@
+import Lean.Elab.Command
+import Lean.Elab.Tactic.ElabTerm
+import Lean.Elab.Tactic.Meta
+import Lean.Meta.CheckTactic
+import Lean.Parser.Term
+
+open Lean Meta Elab Term Command CheckTactic
+
+/-
+This module defines a term generation and testing framework that
+checks whether generated terms have a specified normal form.  It
+is defined in the `Lean.Test.NormalForms` namespace.
+
+To use it, you need to define a few things:
+
+1. a new datatype for representing terms in the language
+2. a data type for representing types
+3. a function for computing the type from the term
+4. a function for rendering the term into Lean syntax
+5. an evaluation function for producing the expected normal form from the term syntax
+6. a list of variable generators for generating variables with different types in the language
+7. a list of operators `Op` for building up terms in the language.
+
+Once this is done, you can pass this information into
+`testNormalForms`.
+-/
+namespace Lean.Test.NormalForms
+
+-- | A `Op` is a first order operation for generating values with a given type.
+structure Op (tp : Type) (val : Type) where
+  args : Array tp
+  result : tp
+  apply : Array val → val
+ deriving Inhabited
+
+def mkOp (args : List tp) (result : tp) (apply : Array val → val) : Op tp val :=
+  { apply := apply, args := args.toArray, result }
+
+def Op.map (op : Op x val) (f : x → y) : Op y val :=
+  { apply := op.apply, args := op.args.map f, result := f op.result }
+
+/--
+Contextual information needed to generate terms.
+-/
+structure GenCtx (term : Type) where
+  -- Maps type indices to operator for corresponding type.
+  -- Types use type indices.
+  ops : Array (Array (Op Nat term))
+  /-- Maps type indices to variables for that type. -/
+  vars : Array (Array term)
+  /- Operators to use for patterns at top of terms -/
+  topOps : Array (Op Nat term)
+  /- Returns the expected reduction of a term -/
+  expected : term → term
+  /- Predicate that returns true if terms are equal-/
+  eq : term → term → Bool
+  /-- Maximum term size -/
+  maxTermSize : Nat
+  /-- Maximum depth of terms -/
+  maxDepth : Nat
+  /-- Maximum number of variables -/
+  maxVarCount : Nat
+  /- Local context variables defined in -/
+  lctx : LocalContext
+  /- Local instances for variables -/
+  linst : LocalInstances
+
+namespace GenCtx
+
+/-- `var ctx tp idx` returns a term denoting `i`th variable with type `tp`. -/
+def var (ctx : GenCtx term) (tp : Nat) (idx : Nat) : Option term :=
+  if g : tp < ctx.vars.size then
+    let a := ctx.vars[tp]'g
+    if h : idx < a.size then
+      some (a[idx]'h)
+    else
+      none
+  else
+    none
+
+end GenCtx
+
+/-- An operator together with a set of terms to apply to it. -/
+structure PartialApp (term : Type) where
+  /-- Operator to generate -/
+  op : Op Nat term
+  /-- Terms constructed so far -/
+  terms : Array term
+
+namespace PartialApp
+
+def fromOp (op : Op Nat term) : PartialApp term :=
+  { op, terms := .mkEmpty op.args.size }
+
+end PartialApp
+
+/--
+A partial term contains the initial part of a term as constructed from a
+left-to-right preorder traversal.
+
+It stores additional information needed to ensure the ultimate term satisfies
+the generation constraints on term size and number of variables.
+
+The operations for constructing this ensures the term is well-formed
+with respect to the signature and is not a complete term.
+-/
+structure PartialTerm (term : Type) where
+  /-- Stack of partially built term (must be non-empty) -/
+  termStack : Array (PartialApp term)
+  /-- Maximum number of additional operations that may be added. -/
+  remTermSize : Nat
+  /-- Variables used with type index. -/
+  usedVars : Array Nat
+  deriving Inhabited
+
+namespace PartialTerm
+
+/--
+Create an initial partial term from an operator.
+
+If the operator is a constant, then this just returns a complete terms.
+-/
+def init (maxTermSize : Nat) (maxDepth : Nat) (op : Op Nat term) : term ⊕ PartialTerm term :=
+  if op.args.isEmpty then
+    .inl (op.apply #[])
+  else
+    .inr {
+      termStack := #[PartialApp.fromOp op],
+      remTermSize := maxTermSize - (1 + op.args.size),
+      usedVars := #[]
+    }
+
+partial def push (p : PartialTerm term) (t : term) : term ⊕ PartialTerm term :=
+  match p.termStack.back? with
+  | none => .inl t
+  | some { op, terms } =>
+    let p := { p with termStack := p.termStack.pop }
+    let terms := terms.push t
+    if terms.size = op.args.size then
+      let v := op.apply terms
+      push p v
+    else
+      .inr { p with termStack := p.termStack.push { op, terms } }
+
+/-- Push an operator to the stack -/
+def pushOp (p : PartialTerm term) (op : Op Nat term) : PartialTerm term :=
+  { termStack   := p.termStack.push (.fromOp op)
+    remTermSize := p.remTermSize - op.args.size,
+    usedVars := p.usedVars
+  }
+
+end PartialTerm
+
+/--
+Term generator
+-/
+structure TermGen (term : Type) where
+  sofar : Array term := #[]
+  pending : Array (PartialTerm term) := #[]
+  deriving Inhabited
+
+namespace TermGen
+
+/-- Return true if generator will return no more terms. -/
+def isEmpty (s: TermGen term) : Bool := s.sofar.isEmpty && s.pending.isEmpty
+
+def pop (s : TermGen term) : Option (Nat × PartialTerm term × TermGen term) :=
+  if s.pending.isEmpty then
+    .none
+  else
+    let { sofar, pending } := s
+    let next := pending.back
+    let pending := pending.pop
+    match next.termStack.back? with
+    | none =>
+      panic! "Term stack empty"
+    | some app =>
+      let tp := app.op.args[app.terms.size]!
+      some (tp, next, { sofar, pending })
+
+def add (gen : TermGen term)  (val : term ⊕ PartialTerm term) : TermGen term :=
+  let { sofar, pending } := gen
+  match val with
+  | .inl v =>  { sofar := sofar.push v, pending }
+  | .inr p => { sofar, pending := pending.push p }
+
+/-
+`push s next v` adds the result of `next.push v` to the state.
+
+This only adds terms that are irreducible.
+-/
+def push (gen : TermGen term) (ctx : GenCtx term) (next : PartialTerm term) (v : term) : TermGen term :=
+  let exp := ctx.expected v
+  if ctx.eq exp v then
+    gen.add (next.push v)
+  else
+    gen
+
+def pushOp (gen : TermGen term) (ctx : GenCtx term) (next : PartialTerm term) (op : Op Nat term) :=
+  if op.args.isEmpty then
+    gen.push ctx next (op.apply #[])
+  else if op.args.size ≤ next.remTermSize ∧ next.termStack.size + 1 < ctx.maxDepth then
+    { gen with pending := gen.pending.push (next.pushOp op) }
+  else
+    gen
+
+/-- Create state that will explore all terms in context -/
+def addOpInstances (s : TermGen term) (ctx : GenCtx term) (op : Op Nat term) : TermGen term :=
+  s.add (PartialTerm.init ctx.maxTermSize ctx.maxDepth op)
+
+/-- Create state that will explore all terms in context -/
+def init (ctx : GenCtx term) : TermGen term :=
+  ctx.topOps.foldl (init := {}) (·.addOpInstances ctx ·)
+
+end TermGen
+
+/--
+Generate terms until we reach the limit.
+-/
+partial
+def generateTerms
+    (ctx : GenCtx term)
+    (gen : TermGen term)
+    (limit : Nat := 0) :
+    Array term × TermGen term :=
+  if limit > 0 ∧ gen.sofar.size ≥ limit then
+    -- Stop if we hit term limit
+    (gen.sofar, { gen with sofar := #[] })
+  else
+    match gen.pop with
+    | none =>
+      -- stop when out of terms
+      (gen.sofar, { gen with sofar := #[] })
+    | some (tp, next, gen) =>
+      -- Add previously used variables to term
+      let addVar (next : PartialTerm term) (i : Nat) (gen : TermGen term) : TermGen term :=
+            -- If the previous variable i matches type, then add it to generator
+            if next.usedVars[i]! = tp then
+              match ctx.var tp i with
+              | some v => gen.push ctx next v
+              | none => gen
+            else
+              gen
+      let s := next.usedVars.size.fold (init := gen) (addVar next)
+      let s :=
+        let var := next.usedVars.size
+        if var < ctx.maxVarCount then
+          let next := { next with usedVars := next.usedVars.push tp }
+          addVar next var s
+        else
+          s
+      generateTerms ctx (ctx.ops[tp]!.foldl (init := s) (·.pushOp ctx next ·)) limit
+
+/-
+`addScopeVariables` extends the local context and instances with a copy of the
+variables in the scope (which must be non-empty).
+-/
+def addScopeVariables (lctx : LocalContext) (linst : LocalInstances) (scope : Scope) (idx : Nat) :
+    CoreM (LocalContext × LocalInstances × Ident) := do
+  let act := Term.elabBindersEx scope.varDecls fun vars => do pure (vars, ← (read : MetaM Meta.Context))
+  let mctx := { lctx := lctx, localInstances := linst }
+  let (((vars, mctx), _tstate), _mstate) ← act |>.run |>.run mctx
+  if vars.isEmpty then
+    throwError "No variables declared"
+  let fv := vars[0]!.snd |>.fvarId!
+  let rec drop (nm : Name) :=
+        match nm with
+        | .str .anonymous s => pure (.str .anonymous s!"{s}{idx}")
+        | .str nm _ => drop nm
+        | .num nm _ => drop nm
+        | .anonymous => throwError "Anonymous variable declared."
+  let nm ← drop (mctx.lctx.get! fv |>.userName)
+  let lctx := mctx.lctx.setUserName fv nm
+  pure (lctx, mctx.localInstances, mkIdent nm)
+
+def addVariables (cmdCtx : Command.Context) (cmdState : Command.State) (lctx : LocalContext) (linst : LocalInstances) (n : Nat) (cmd : Command) :
+    CoreM (LocalContext × LocalInstances × Array Ident) := do
+  let (_, s) ←  elabCommand cmd.raw |>.run cmdCtx |>.run cmdState
+  let scope := s.scopes.head!
+  Nat.foldM (n := n) (init := (lctx, linst, .mkEmpty n)) fun i (lctx, linst, a) => do
+    let (lctx, linst, ident) ← addScopeVariables lctx linst scope i
+    pure (lctx, linst, a.push ident)
+
+structure GenStats where
+  maxTermSize : Nat := 9
+  maxDepth : Nat := 3
+  maxVarCount : Nat := 3
+
+
+structure VarDecl (tp : Type) where
+  idx : Nat
+  ident : TSyntax `ident
+  type : tp
+  deriving Inhabited, Repr
+
+instance : BEq (VarDecl tp) where
+  beq x y := x.idx == y.idx
+
+instance : Hashable (VarDecl tp) where
+  hash v := hash v.idx
+
+/--
+
+-/
+class GenTerm (term : Type) (type : outParam Type) extends BEq term where
+  mkVar : VarDecl type → term
+  render : term → TermElabM Term
+
+def mkCtx [BEq tp] [Hashable tp] [BEq term]
+    (types : Array tp)
+    (ops : List (Op tp term))
+    (varGen : List (tp × CoreM Command))
+    (mkVar : VarDecl tp → term)
+    (expected : term → term)
+    (stats : GenStats)
+    (topOps : List (Op tp term) := ops) : CommandElabM (GenCtx term) := do
+  let typeMap : HashMap tp Nat := Nat.fold (n := types.size) (init := {}) fun i s =>
+        if p : i < types.size then
+          s.insert types[i] i
+        else
+          s
+  let typeFn (t : tp) := typeMap.findD t 0
+  let addOp (a : Array (Array (Op Nat term))) (op : Op tp term) :=
+        let op := op.map typeFn
+        a.modify op.result (·.push op)
+  let init := Array.ofFn (n := types.size) (fun _ => #[])
+  let ops := ops.foldl (init := init) addOp
+  let ops := ops.map (·.reverse)
+  let topOps := topOps.toArray.map (·.map typeFn)
+  let (lctx, linst, vars) ← liftCoreM do
+    let coreCtx ← read
+    let coreState ← get
+    let fileName := coreCtx.fileName
+    let fileMap  := coreCtx.fileMap
+    let env := coreState.env
+    let maxRecDepth := coreCtx.maxRecDepth
+    let cmdCtx : Command.Context := { fileName, fileMap, tacticCache? := none }
+    let cmdState : Command.State := { env, maxRecDepth }
+    let addVars (p : LocalContext × LocalInstances × Array (Array term))
+                (q : tp × CoreM Command) :
+                CoreM (LocalContext × LocalInstances × _) := do
+          let (lctx, linst, a) := p
+          let (type, gen) := q
+          let cmd ← gen
+          let (lctx, linst, vars) ← addVariables cmdCtx cmdState lctx linst stats.maxVarCount cmd
+          let vars := Array.ofFn (n := vars.size) fun j => mkVar { idx := j.val, ident := vars[j], type }
+          let type := typeFn type
+          pure (lctx, linst, a.modify type (fun _ => vars))
+    let vars := Array.ofFn (n := types.size) fun _ => #[]
+    varGen.foldlM (init := ({}, {}, vars)) addVars
+  let maxTermSize : Nat := stats.maxTermSize
+  let maxDepth : Nat := stats.maxDepth
+  let maxVarCount : Nat := stats.maxVarCount
+  pure { ops, vars, expected := @expected, eq := BEq.beq, topOps, maxTermSize, maxDepth, maxVarCount, lctx, linst }
+
+/-
+runTest
+-/
+def runTest (render : term → TermElabM Syntax.Term) (simp : term → term) (tac : Syntax.Tactic) (tm : term) : TermElabM Unit := do
+  withoutModifyingEnv $ do
+    let res := simp tm
+    let t ← render tm
+    let exp ← render res
+    let u ← Lean.Elab.Term.elabTerm t none
+    let type ← inferType u
+    let checkGoalType ← mkCheckGoalType u type
+    let expTerm ← Lean.Elab.Term.elabTerm exp (some type)
+    let mvar ← mkFreshExprMVar (.some checkGoalType)
+    let (goals, _) ← Lean.Elab.runTactic mvar.mvarId! tac.raw
+    match goals with
+    | [next] => do
+      let (val, _, _) ← matchCheckGoalType (←next.getType)
+      if !(← Meta.withReducible <| isDefEq val expTerm) then
+        logError m!"{indentExpr u} reduces to{indentExpr val}\nbut is expected to reduce to {indentExpr expTerm}"
+    | [] =>
+      logError m!"{tac} closed goal, but is expected to reduce to {indentExpr expTerm}."
+    | _ =>
+      logError m!"{tac} produced multiple goals, but is expected to reduce to {indentExpr expTerm}."
+
+/-
+Create core context for running tactic tests in.
+-/
+private def mkCoreContext (ctx : Command.Context) (options : Options) (maxRecDepth : Nat) (initHeartbeats : Nat) : Core.Context :=
+  { fileName       := ctx.fileName
+    fileMap        := ctx.fileMap
+    options,
+    currRecDepth   := ctx.currRecDepth
+    maxRecDepth,
+    ref            := ctx.ref
+    initHeartbeats,
+    currMacroScope := ctx.currMacroScope }
+
+/-- Runs term elaborator in base context. -/
+def runTermElabM (cctx : Core.Context) (cstate : Core.State) (mctx : Meta.Context) (act : TermElabM Unit)
+    : BaseIO (Except Exception MessageLog) := do
+  let r ← act.run |>.run mctx |>.run cctx cstate |>.toBaseIO
+  match r with
+  | .error e =>
+    pure (.error e)
+  | .ok ((((), _termS), _metaS), coreS) =>
+    pure (.ok coreS.messages)
+
+/--
+Tests that a tactic applied to exhaustively generated terms matches
+expectations.
+
+To allow testing consistent treatment of operators on multiple types, the normal
+form testing facility is defined using terms over an arbitrary simply-typed
+`term` data type that uses types using the `type` parameter.  This
+representation should be chosen to make specifying the semantics of the tactic
+as simple as possible.
+
+Term must be an instance of the `GenTerm` class so the testing facility knows
+how to render user terms into Lean terms.  Additionally, users should provide
+operators and variable constructors for building terms up.
+
+`stats` controls parameters on the size of terms generated.
+-/
+partial def testNormalForms {val type : Type} [BEq type] [Hashable type] [GenTerm val type]
+      (types : List type)
+      (ops : List (Op type val))
+      (vars : List (type × CoreM Command))
+      (expected : val → val)
+      (stats : GenStats)
+      (tac : Option Syntax.Tactic := none)
+      (topOps : List (Op type val) := ops)
+      (concurrent : Bool := true) : CommandElabM Unit := do
+
+  let tac ← tac.getDM `(tactic|try simp)
+  let ctx ← mkCtx (types := types.toArray) (ops := ops) (topOps := topOps) (varGen := vars) (mkVar := GenTerm.mkVar) expected (stats := stats)
+
+  let cmdCtx : Command.Context ← read
+  let s ← get
+  let maxRecDepth := s.maxRecDepth
+  let heartbeats ← IO.getNumHeartbeats
+  let options ← getOptions
+  -- Create core context for running tests.
+  let cctx := mkCoreContext cmdCtx options maxRecDepth heartbeats
+  -- Create core context for running tests.
+  let cstate : Core.State := {
+        env := s.env,
+        ngen := s.ngen,
+        traceState := s.traceState,
+        infoState.enabled := s.infoState.enabled
+    }
+  -- Meta context setup for variables created by mkCtx
+  let mctx : Meta.Context := { lctx := ctx.lctx, localInstances := ctx.linst }
+  let gen := TermGen.init ctx
+  if concurrent then
+    let limit := 800
+    let rec loop (gen : TermGen val) (cnt : Nat) (tasks : Array (Task (Except Exception MessageLog))) : BaseIO (Nat × Array (Task _)) := do
+      if gen.isEmpty then
+        return (cnt, tasks)
+      else
+        let (terms, gen) := generateTerms ctx gen (limit := limit)
+        let runTests := do
+              for tm in terms do
+                if ← IO.checkCanceled then
+                  break
+                runTest GenTerm.render expected tac tm
+        let t ← runTests |> runTermElabM cctx cstate mctx |>.asTask
+        loop gen (cnt + terms.size) (tasks.push t)
+    let (cnt, tasks) ←
+      profileitM Exception "normal form generation" (←getOptions) (decl := .anonymous) do
+        liftIO (loop gen 0 #[])
+    trace[Test.normalforms] "generated {cnt} tests running in {tasks.size} threads."
+    profileitM Exception "normal form execution" (←getOptions) do
+      for i in [0:tasks.size] do
+        if ← IO.checkCanceled then
+          break
+        let act := tasks[i]!
+        match act.get with
+        | .error e =>
+          -- Cancel all tasks after this one
+          (tasks |>.toSubarray (start := i+1) |>.forM IO.cancel : BaseIO Unit)
+          throw e
+        | .ok m =>
+          modify fun s => { s with messages := s.messages ++ m }
+  else
+    let r ← runTermElabM cctx cstate mctx <|
+      let (terms, _) := generateTerms ctx gen (limit := 0)
+      for tm in terms do
+        if ← IO.checkCanceled then
+          break
+        runTest GenTerm.render expected tac tm
+    match r with
+    | .error e => throw e
+    | .ok m => modify fun s => { s with messages := s.messages ++ m }
+
+builtin_initialize
+  registerTraceClass `Test.normalforms
+
+end Lean.Test.NormalForms
