tests/playground/int_exhaust_test.lean
@@ -1,0 +1,624 @@
+import Lean.Util.TestNormalForms
+import Lean.Meta.Tactic.Simp.BuiltinSimprocs
+import Lean.Meta.LitValues
+
+open Lean
+open Lean.Elab.Command (CommandElab)
+open Lean.Test.NormalForms
+
+namespace Nat
+
+attribute [simp] mod_one
+
+theorem succ_mod_bad (a b : Nat) : (a + 1) % b = if b ∣ (a + 1) then 0 else (a % b) + 1 := by
+  split
+  · rename_i dp
+    apply Nat.mod_eq_zero_of_dvd dp
+  · rename_i dp
+    match b with
+    | 0 =>
+      simp
+    | 1 =>
+      simp at dp
+    | b + 2 =>
+      revert dp
+      rw [Nat.dvd_iff_mod_eq_zero, ←Nat.mod_mod (a+1) _, ←Nat.mod_mod a _, Nat.add_mod a 1 _]
+      have p : 1 < b + 2 := Nat.le_add_left _ _
+      simp only [Nat.mod_eq_of_lt p]
+      have qle : a % (b + 2) + 1 ≤ b + 2 := by apply Nat.mod_lt _ (Nat.zero_lt_succ _)
+      match Nat.lt_or_eq_of_le qle with
+      | .inl p =>
+        simp [Nat.mod_eq_of_lt p]
+      | .inr q =>
+        simp [q]
+
+theorem succ_mod (a b : Nat) : (a + 1) % b = if a % b + 1 = b then 0 else (a % b) + 1 := by
+  match b with
+  | 0 =>
+    simp
+  | 1 =>
+    simp
+  | b + 2 =>
+    simp only [Nat.succ.injEq]
+    split
+    · rename_i dp
+      rw [Nat.add_mod a 1 _]
+      simp [dp]
+    · rename_i dp
+      have one_lt : 1 < b + 2 := Nat.le_add_left ..
+      have q : a % (b + 2) ≤ b + 1 := Nat.le_of_succ_le_succ (Nat.mod_lt _ (by omega))
+      have a_lt : a % (b + 2) + 1 < b + 2 := Nat.succ_lt_succ (Nat.lt_of_le_of_ne q dp)
+      rw [Nat.add_mod a 1 _]
+      rw [Nat.mod_eq_of_lt one_lt, Nat.mod_eq_of_lt a_lt]
+
+#print Nat.add_sub_add_left
+
+theorem sub_div {x n : Nat} (h : n ≤ x) : (x - n) / n = x / n - 1 := by
+  have sd := Nat.sub_mul_div x n 1
+  simp [Nat.mul_one] at sd
+  exact sd h
+
+theorem eq_sub_iff (a : Nat) {b c : Nat} (p : b ≥ c) : (a = b - c) ↔ (a + c = b) := by
+  rw [@Eq.comm _ a, Nat.sub_eq_iff_eq_add p, @Eq.comm _ b]
+
+theorem succ_div_d (a b : Nat) : (a + 1) / b =
+    if b ∣ (a+1) then a / b + 1 else a / b := by
+  match b with
+  | 0 =>
+    simp
+  | 1 =>
+    simp
+  | b + 2 =>
+    admit
+
+theorem succ_div (a b : Nat) : (a + 1) / b =
+    if b * (a / b + 1) = a + 1 then a / b + 1 else a / b := by
+  match b with
+  | 0 =>
+    simp
+  | 1 =>
+    simp
+  | b + 2 =>
+    rw [div_eq]
+    have h : Decidable (b + 1 < a) := inferInstance
+    cases h with
+    | isFalse h =>
+      if ne : a = b + 1 then
+        have lts : b+1 < b + 2 := Nat.lt_succ_self (b+1)
+        simp [Nat.succ_le_succ_iff, ne, Nat.div_eq_of_lt lts]
+      else
+        have lt : a < b + 2 := Nat.lt_of_not_le h
+        have lt3 := Nat.lt_of_le_of_ne (Nat.le_of_lt_succ lt) ne
+        simp [Nat.succ_le_succ_iff, Nat.not_le_of_lt lt3, Nat.div_eq_of_lt lt, Ne.symm ne]
+    | isTrue h =>
+      have a_ge : b + 2 ≤ a := h
+      have a1_ge : b + 2 ≤ a + 1 := Nat.succ_le_succ (Nat.le_of_succ_le h)
+      simp [Nat.zero_lt_succ, a1_ge]
+
+      have sd := Nat.sub_mul_div a (b+2) 1
+      simp [Nat.mul_one] at sd
+      replace sd := sd h
+
+      have lhs_eq : a - (b + 2) + 1 = a - (b + 1) := by omega
+      have a_div_pos : a / (b + 2) ≥ 1 := by admit
+      have ih := succ_div (a - (b+2)) (b+2)
+      simp only [lhs_eq, sub_div a_ge, Nat.sub_add_cancel a_div_pos] at ih
+      rw [ih]
+      simp [Nat.mul_add, Nat.eq_sub_iff _ (Nat.le_of_lt h), ←Nat.add_assoc, Nat.succ_inj']
+      split
+      · simp
+      · simp [Nat.sub_add_cancel a_div_pos]
+
+/-
+theorem foo (a b n : Nat) : n ∣ a - n * b ↔ (n ∣ a) := by
+  apply Iff.intro
+  · intro p
+    have q := Nat.dvd_def n a
+    rw [Nat.dvd_def n a] at p
+    admit
+  · admit
+-/
+
+end Nat
+
+namespace Int
+
+attribute [simp] emod_self
+
+--@[simp] theorem zero_bdiv : bdiv 0 n = 0 := by sorry
+
+--@[simp] theorem bdiv_one : bdiv m 1 = 0 := by sorry
+
+@[simp] theorem zero_bdiv (n : Nat) : bdiv 0 n = 0 := by
+  unfold bdiv; simp; omega
+@[simp] theorem bdiv_zero  (n : Int) : bdiv n 0 = 0 := by rfl
+
+@[simp] theorem bdiv_one   (n : Int) : bdiv n 1 = n := by unfold bdiv; simp
+
+@[simp] theorem bmod_zero (n : Int) : bmod n 0 = n := by unfold bmod; simp
+
+example : Int.mod m (-n) = Int.mod m n := by simp
+
+--example : Int.fmod m (-n) = -(Int.fmod m n) := by
+
+section
+open Lean.Meta Simp
+
+def reduceBinIntNatOp (name : Name) (op : Int → Nat → Int) (e : Expr) : SimpM DStep := do
+  unless e.isAppOfArity name 2 do return .continue
+  let some v₁ ← getIntValue? e.appFn!.appArg! | return .continue
+  let some v₂ ← getNatValue? e.appArg! | return .continue
+  return .done <| toExpr (op v₁ v₂)
+
+dsimproc [simp, seval] reduceTDiv (Int.div _ _) := reduceBin ``Int.div 2 Int.div
+dsimproc [simp, seval] reduceTMod (Int.mod _ _) := reduceBin ``Int.mod 2 Int.mod
+dsimproc [simp, seval] reduceFDiv (Int.fdiv _ _) := reduceBin ``Int.fdiv 2 Int.fdiv
+dsimproc [simp, seval] reduceFMod (Int.fmod _ _) := reduceBin ``Int.fmod 2 Int.fmod
+dsimproc [simp, seval] reduceBdiv (bdiv _ _) := reduceBinIntNatOp ``bdiv bdiv
+dsimproc [simp, seval] reduceBmod (bmod _ _) := reduceBinIntNatOp ``bmod bmod
+
+end
+
+
+set_option trace.Meta.Tactic.simp true
+
+example : bdiv 1 1 = 1 := by
+  simp
+
+end Int
+
+inductive NumType where
+| nat
+| int
+deriving BEq, Hashable, Inhabited, Repr
+
+protected def NumType.render [Monad M] [MonadQuotation M] (v : NumType) : M Term := do
+  match v with
+  | nat => `(Nat)
+  | int => `(Int)
+
+inductive  DivMode where
+  | divNat
+  | edivInt
+  | fdivInt
+  | tdivInt
+  | bdivInt
+  deriving BEq, Repr
+
+def DivMode.typeOf (m : DivMode) : NumType :=
+  match m with
+  | divNat => .nat
+  | edivInt => .int
+  | fdivInt => .int
+  | tdivInt => .int
+  | bdivInt => .int
+
+inductive NumTerm where
+  | var (d : VarDecl NumType)
+  | lit (n : Nat) (tp : NumType)
+  | natToInt (x : NumTerm)
+  | intToNat (x : NumTerm)
+  | add (x y : NumTerm) (tp : NumType)
+  | sub (x y : NumTerm) (tp : NumType)
+  | neg (x : NumTerm)
+  | mul (x y : NumTerm) (tp : NumType)
+  | div (x y : NumTerm) (m : DivMode)
+  | mod (x y : NumTerm) (m : DivMode)
+  deriving BEq, Inhabited, Repr
+
+namespace NumTerm
+
+open NumType
+
+partial def map (f : NumTerm → NumTerm) (v : NumTerm) : NumTerm :=
+  match v with
+  | var _ | lit _ _ => v
+  | natToInt x => natToInt (f x)
+  | intToNat x => intToNat (f x)
+  | add x y tp => add (f x) (f y) tp
+  | sub x y tp => sub (f x) (f y) tp
+  | neg x => neg (f x)
+  | mul x y tp => mul (f x) (f y) tp
+  | div x y op => div (f x) (f y) op
+  | mod x y op => mod (f x) (f y) op
+
+protected def typeOf (v : NumTerm) : NumType :=
+  match v with
+  | var d => d.type
+  | lit _ tp => tp
+  | natToInt _ => .int
+  | intToNat _ => .nat
+  | add _ _ tp => tp
+  | sub _ _ tp => tp
+  | neg _ => .int
+  | mul _ _ tp => tp
+  | div _ _ op => op.typeOf
+  | mod _ _ op => op.typeOf
+
+protected def render [Monad M] [MonadQuotation M] (v : NumTerm) : M Term := do
+  match v with
+  | var d => pure d.ident
+  | lit n tp => `(($(Syntax.mkNumLit (toString n)) : $(←tp.render)))
+  | natToInt x => `((($(←x.render) : Nat) : Int))
+  | intToNat x => `((($(←x.render) : Int) : Nat))
+  | add x y tp => `((($(←x.render) + $(←y.render)) : $(←tp.render)))
+  | sub x y _ => `($(←x.render) - $(←y.render))
+  | neg x => `(- $(←x.render))
+  | mul x y _ => `($(←x.render) * $(←y.render))
+  | div x y op =>
+    match op with
+    | .divNat  => `($(←x.render) / $(←y.render))
+    | .edivInt => `($(←x.render) / $(←y.render))
+    | .fdivInt => `(Int.fdiv $(←x.render) $(←y.render))
+    | .tdivInt => `(Int.div  $(←x.render) $(←y.render))
+    | .bdivInt => `(Int.bdiv $(←x.render) $(←y.render))
+  | mod x y op =>
+    match op with
+    | .divNat  => `($(←x.render) % $(←y.render))
+    | .edivInt => `($(←x.render) % $(←y.render))
+    | .fdivInt => `(Int.fmod $(←x.render) $(←y.render))
+    | .tdivInt => `(Int.mod  $(←x.render) $(←y.render))
+    | .bdivInt => `(Int.bmod $(←x.render) $(←y.render))
+
+instance : GenTerm NumTerm NumType where
+  render := NumTerm.render
+  mkVar := NumTerm.var
+
+def intLit (i : Int) : NumTerm :=
+  if i < 0 then
+    neg (lit ((- i).toNat) .int)
+  else
+    lit i.toNat .int
+
+def asIntLit (i : NumTerm) : Option Int :=
+  match i with
+  | .lit n _ => some (n : Int)
+  | .neg (.lit n .int) => some (- (n : Int))
+  | _ => none
+
+partial def simp (v : NumTerm) : NumTerm :=
+  let v := map simp v
+  match v with
+  | natToInt x =>
+    (match x with
+    | lit n _ => lit n .int
+    | add x y _ => add (natToInt x) (natToInt y) .int
+    | mul x y _ => mul (natToInt x) (natToInt y) .int
+    | div x y _ => div (natToInt x) (natToInt y) .edivInt
+    | mod x y _ => mod (natToInt x) (natToInt y) .edivInt
+    | var _ | sub _ _ _ | neg _ | intToNat _ | natToInt _ => v)
+  | add x y tp =>
+    match x, y with
+    | x, lit 0 _ => x
+    | lit 0 _, y => y
+    | lit i _, lit j _ => lit (i+j) tp
+    | _, _ => v
+  | sub x y tp =>
+    match x, y, tp with
+    | x, lit 0 _, _ => x
+    | lit i _, lit j _, .nat => lit (i-j) tp
+    | lit i _, lit j _, .int => intLit ((i : Int) - (j : Int))
+    | lit 0 _, _, .nat => lit 0 .nat
+    | lit 0 _, y, .int => simp (neg y)
+    | x, y, _ =>
+      if x == y then
+        .lit 0 tp
+      else
+        v
+  | neg x =>
+    match x with
+    | lit n _ => intLit (- (Int.ofNat n))
+    | _ => v
+  | mul x y tp =>
+    match x, y with
+    | _, lit 0 _ => y
+    | lit 0 _, _ => x
+    | _, lit 1 _ => x
+    | lit 1 _, _ => y
+    | lit i _, lit j _ => lit (i*j) tp
+    | _, _ => v
+  | div x y op =>
+    if let (some x, some y) := (asIntLit x, asIntLit y) then
+      match op with
+      | .divNat => lit (Nat.div x.toNat y.toNat) .nat
+      | .edivInt => intLit (Int.ediv x y)
+      | .fdivInt => intLit (Int.fdiv x y)
+      | .tdivInt => intLit (Int.div  x y)
+      | .bdivInt => intLit (Int.bdiv x y.toNat)
+    else if let lit 0 _ := x then
+      x
+    else if let lit 0 _ := y then
+      y
+    else if let lit 1 _ := y then
+      x
+    else
+      v
+  | mod x y op =>
+    if let (some x, some y) := (asIntLit x, asIntLit y) then
+      match op with
+      | .divNat => lit (Nat.mod x.toNat y.toNat) .nat
+      | .edivInt => intLit (Int.emod x y)
+      | .fdivInt => intLit (Int.fmod x y)
+      | .tdivInt => intLit (Int.mod  x y)
+      | .bdivInt => intLit (Int.bmod x y.toNat)
+    else if let lit 0 _ := x then
+      x
+    else if let lit 0 _ := y then
+      x
+    else if let lit 1 _ := y then
+      lit 0 op.typeOf
+    else if x == y then
+      lit 0 op.typeOf
+    else Id.run do
+      if let mul xa xb tp := x then
+        if xa == y || xb == y then
+          return lit 0 tp
+      if let mod xn xd _xop := x then
+        if xd == y then
+          return simp (mod xn y op)
+      if let neg yn := y then
+        match op with
+        | .edivInt | .tdivInt | .bdivInt =>
+          return simp (mod x yn op)
+        | _ =>
+          pure ()
+      return v
+  | _ => v
+
+partial def simpv (u : NumTerm) : NumTerm :=
+  let v := simp u
+  if v.typeOf == u.typeOf then
+    v
+  else
+    panic! s!"{repr u} has changed types."
+
+def litOp (n : Nat) (tp : NumType) := mkOp [] tp fun _ => lit n tp
+def addOp (tp : NumType) := mkOp [tp, tp] tp fun a => add (a[0]!) (a[1]!) tp
+def subOp (tp : NumType) := mkOp [tp, tp] tp fun a => sub (a[0]!) (a[1]!) tp
+def negOp : Op NumType NumTerm := mkOp [.int] .int fun a => neg (a[0]!)
+def mulOp (tp : NumType) := mkOp [tp, tp] tp fun a => mul (a[0]!) (a[1]!) tp
+def divOp (op : DivMode) (dtp := op.typeOf) := let tp := op.typeOf; mkOp [tp, dtp] tp fun a => div (a[0]!) (a[1]!) op
+def modOp (op : DivMode) (dtp := op.typeOf) := let tp := op.typeOf; mkOp [tp, dtp] tp fun a => mod (a[0]!) (a[1]!) op
+
+end NumTerm
+
+open NumTerm
+
+syntax:lead (name := intTestElab) "#intTest" : command
+
+@[command_elab intTestElab]
+def elabIntTest : CommandElab := fun _stx => do
+  let types : List NumType := [.nat, .int]
+  let ops := [
+      litOp 0 .nat,
+      litOp 1 .nat,
+      litOp 2 .nat,
+      litOp 0 .int,
+      litOp 1 .int,
+      litOp 2 .int,
+      addOp .nat, addOp .int,
+      subOp .nat, subOp .int,
+      negOp,
+      mulOp .nat, mulOp .int,
+      divOp .divNat, divOp .edivInt, divOp .fdivInt, divOp .tdivInt, divOp .bdivInt .nat,
+      modOp .divNat, modOp .edivInt, modOp .fdivInt, modOp .tdivInt, modOp .bdivInt .nat,
+  ]
+  let vars : List (NumType × CoreM Command) := [
+      (.nat, `(variable (n : Nat))),
+      (.int, `(variable (i : Int)))
+  ]
+  let stats : GenStats := { maxTermSize := 6, maxDepth := 3, maxVarCount := 2 }
+  testNormalForms types ops vars NumTerm.simpv stats
+
+set_option maxHeartbeats 100000000
+set_option pp.coercions false
+--set_option pp.explicit true
+--#intTest
+
+
+namespace Int
+
+theorem emod_lt (a b : Int) (h : b ≠ 0) : a % b < Int.natAbs b := by
+  rw [emod_as_nat_mod]
+  if p : a ≥ 0 then
+    simp [p, -Int.ofNat_emod]
+    exact Nat.mod_lt _ (by omega)
+  else
+    simp [p, -Int.ofNat_emod]
+    apply Int.sub_lt_self
+    apply Int.succ_ofNat_pos
+
+
+--set_option pp.explicit true
+
+theorem div_as_nat (x y : Int) : Int.div x y =
+  ite (x ≥ 0) 1 (-1) * ite (y ≥ 0) 1 (-1) * ((x.natAbs) / (y.natAbs)) := by
+  cases x <;> cases y <;>  simp [Int.div, ofNat_nonneg, ←Int.neg_eq_neg_one_mul]
+
+#print Int.emod
+
+theorem emod_ofNat   (a : Nat) (b : Int) : Nat.cast a % b = Nat.cast (a % b.natAbs) := rfl
+theorem emod_negSucc (a : Nat) (b : Int) : -[a+1] % b = (b.natAbs : Int) - (a % b.natAbs + 1) := rfl
+
+/-
+def emod : (@& Int) → (@& Int) → Int
+  | ofNat m, n => ofNat (m % natAbs n)
+  | -[m+1],  n => subNatNat (natAbs n) (succ (m % natAbs n))
+-/
+
+set_option trace.Meta.Tactic.simp.rewrite true
+
+#print Int.ediv
+
+#print Int.div
+
+theorem ediv_ofNat_negSucc (m n : Nat) : m / -[n+1] = -ofNat (m / Nat.succ n) := rfl
+theorem ediv_negSucc_zero (m : Nat) : -[m+1] / 0 = 0 := rfl
+theorem ediv_negSucc_succ (m n : Nat) : -[m+1] / (n + 1 : Nat) = -((m / (n + 1)) : Nat) + (-1) := by
+  simp [HDiv.hDiv, Div.div, Int.ediv, Int.negSucc_coe']
+  admit
+theorem ediv_negSucc_negSucc (m n : Nat) : -[m+1] / -[n+1] = ((m / (n + 1) + 1) : Nat) := rfl
+
+theorem ofNat_not_neg (a : Nat) : (a : Int) < 0 ↔ False := by
+  simp only [iff_false]
+  apply Int.not_le_of_gt
+  simp [Int.add_le_add_iff_left]
+
+--set_option pp.explicit true
+
+theorem dvd_natCast_negSucc (a b : Nat) : (a : Int) ∣ -[ b +1] ↔ a ∣ b+1 := by
+  simp [Int.dvd_iff_mod_eq_zero, Nat.dvd_iff_mod_eq_zero, mod, Int.emod_ofNat,
+    -emod_ofNat]
+  apply Int.ofNat_inj
+
+theorem dvd_negSucc_negSucc (a b : Nat) : -[a +1] ∣ -[ b +1] ↔ a+1 ∣ b+1 := by
+  simp [Int.dvd_iff_mod_eq_zero, Nat.dvd_iff_mod_eq_zero, mod, Int.emod_ofNat,
+    -emod_ofNat]
+  apply Int.ofNat_inj
+
+theorem div_eq_ediv' (a b : Int) : Int.div a b = a / b + ite (a < 0 ∧ ¬(b ∣ a)) (sign b) 0  :=
+  match a, b with
+  | (a : Nat), ofNat b => rfl
+  | (a : Nat), -[b +1] => by
+    simp [Int.div, ediv_ofNat_negSucc, ofNat_not_neg]
+  | -[a +1], 0 => by
+    simp [Int.div, ediv_negSucc_zero]
+  | -[a +1], (b+1 : Nat) => by
+    have q : ¬(Nat.cast ((b + 1) : Nat) = (0 : Int)) := by
+      norm_cast
+    simp [-Int.natCast_add] at q
+    simp [Int.div, ediv_negSucc_succ, Nat.succ_div_d,
+          Int.negSucc_lt_zero, q, true_and,  dvd_natCast_negSucc,
+          -Int.natCast_add]
+    split <;> rename_i pg
+    · simp [Int.neg_add]
+    · simp [Int.neg_add, Int.neg_add_cancel_right]
+  | -[m +1], -[n +1] => by
+    simp [Int.div, ediv_negSucc_negSucc,
+      dvd_negSucc_negSucc,
+      Int.negSucc_lt_zero,
+      -ofNat_ediv, -natCast_add,
+      Nat.succ_div_d]
+    simp only [Nat.succ_eq_add_one]
+    split <;> rename_i h
+    . simp
+    · simp [Int.add_neg_cancel_right]
+
+theorem mod_eq_emod' (a b : Int) : Int.mod a b = a % b - b * ite (a < 0 ∧ ¬(b ∣ a)) (sign b) 0 := by
+  simp [emod_def, mod_def, div_eq_ediv',
+        Int.mul_add, Int.sub_eq_add_neg, Int.neg_add, Int.add_assoc]
+
+theorem mod_as_nat_mod (a b : Int) :
+  Int.mod a b =
+    (ite (a ≥ 0) 1 (-1)) * ((a.natAbs % b.natAbs : Nat) : Int) :=
+  match a, b with
+  | ofNat a, ofNat b => by
+    simp [Int.mod, Int.ofNat_nonneg]
+  | ofNat a, -[b +1] => by
+    simp [Int.mod, Int.ofNat_nonneg]
+  | -[a +1], ofNat b => by
+    simp [Int.mod, ←Int.neg_eq_neg_one_mul]
+  | -[m +1], -[n +1] => by
+    simp [Int.mod, ←Int.neg_eq_neg_one_mul, -Int.ofNat_emod]
+
+set_option maxHeartbeats 100000000
+
+-- This is false because a % b is non-neg
+-- We do not prove Int.mod (a % b) b as (a % b) is non-neg
+
+
+--@[simp] theorem add_mod_self {a b : Int} : Int.mod(a + b)  b = a % b := by
+--  have := add_mul_emod_self_left a b 1; rwa [Int.mul_one] at this
+
+@[simp]
+theorem dvd_sub_natAbs (a b : Int) : (a ∣ (b - a.natAbs)) ↔ a ∣ b := by sorry
+
+@[simp]
+theorem dvd_mod_self (a b : Int) : (a ∣ (b % a)) ↔ a ∣ b := by sorry
+
+#eval Int.mod (-3) 2
+#eval Int.mod (-1) 2
+
+@[simp]
+theorem mod_lt_iff (a b : Int) : a % b < b.natAbs ↔ b.natAbs > 0 := by sorry
+
+theorem sub_lt_iff (a b c : Int) : a - b < c ↔ a < c + b := by
+  sorry
+
+theorem emod_neg_iff (m n : Int) : m % n < 0 ↔ m < 0 ∧ n = 0 := by
+  admit
+
+theorem emod_sub_natAbs_self (m n : Int) : (m - n.natAbs) % n = m % n := by
+  simp [←Int.mul_sign, Int.sub_eq_add_neg, Int.neg_mul_eq_mul_neg]
+
+theorem mod_emod (m n : Int) : Int.mod (m % n) n = m % n := by
+  simp_all [mod_eq_emod', emod_neg_iff]
+
+theorem mod_mod (m n : Int) : Int.mod (Int.mod m n) n = Int.mod m n := by
+  simp only [mod_eq_emod' m n]
+  split
+  · rename_i mnn
+    rw [mod_eq_emod']
+    by_cases (OfNat.ofNat 0 < natAbs n) <;>
+    simp_all [sub_lt_iff, Int.mul_sign, emod_sub_natAbs_self]
+  · simp [mod_emod]
+
+theorem negSucc_in_add (a b : Nat) : -[a + b +1] = -[a+1] - b := by
+  cases b <;> rfl
+
+theorem fmod_as_nat_mod (a b : Int) :
+  Int.fmod a b =
+    let d := a ≥ 0 ↔ b ≥ 0
+    let r := ((a.natAbs % b.natAbs : Nat) : Int)
+    ite (a ≥ 0) 1 (-1) * r +
+      (if b ∣ a ∨ d then 0 else b) :=
+  match a, b with
+  | 0, b => by
+    simp [Int.fmod, Int.le_refl, Int.dvd_zero]
+  | ofNat (a+1), ofNat b => by
+    simp [Int.fmod, Int.ofNat_nonneg, -Int.natCast_add]
+  | ofNat (a+1), -[b +1] => by
+    simp [Int.fmod, Int.ofNat_nonneg,
+      -Int.natCast_add, ←Int.natAbs_dvd_natAbs, -Int.ofNat_emod]
+    match b with
+    | 0 =>
+      simp [subNatNat_self]
+    | b + 1 =>
+      -- Cleanup
+      have bnorm : Nat.succ (b + 1) = b + 2 := rfl
+      simp only [←Int.neg_eq_neg_one_mul, bnorm]
+      simp [←Int.ofNat_add_negSucc, -Int.ofNat_emod]
+      rw [Nat.succ_mod]
+      simp only [Nat.succ_inj']
+      split
+      · rename_i pq
+        simp [Nat.dvd_iff_mod_eq_zero, Nat.succ_mod, pq,
+              Int.ofNat_add_negSucc, Int.subNatNat_self,
+              -Int.natCast_add, -Int.ofNat_emod]
+      · rename_i pq
+        simp [Nat.dvd_iff_mod_eq_zero,
+          Nat.succ_mod, Nat.succ_inj', pq,
+          -Int.ofNat_emod, Int.natCast_add]
+        have ns : -[b + 1 +1] = -[b +1] + (-1) := rfl
+        simp only [ns, Int.add_comm -[b +1] (-1), ←Int.add_assoc,
+          Int.add_neg_cancel_right]
+  | -[a +1], ofNat b => by
+    simp [←Int.neg_eq_neg_one_mul,
+      Int.fmod, ofNat_emod, Int.ofNat_nonneg, Int.subNatNat_eq_coe,
+      -Int.ofNat_emod]
+    simp only [Int.dvd_iff_emod_eq_zero, Int.emod_as_nat_mod]
+
+    norm_cast
+    admit
+  | -[m +1], -[n +1] => by
+    simp [Int.fmod, ←Int.neg_eq_neg_one_mul]
+
+
+--theorem tmod_fmod (m n : Int) : Int.mod (Int.fmod m n) n = Int.mod m n := by
+--  admit
+
+-- This is false because a % b is non-neg
+--theorem tmod_emod (a b : Int) : Int.bmod (a % b) b = Int.mod a b := by
+--  admit
+
+end Int
